**BINOMIAL THEOREM:**
--
![(a+b)^n = \sum_{k=0}^{n}( ^{n}_{k})a^{n-k}b^{k}](https://latex.codecogs.com/svg.image?\bg_white&space;(a&plus;b)^n&space;=&space;\sum_{k=0}^{n}(&space;^{n}_{k})a^{n-k}b^{k})    where    ![( ^{n}_{k})= \frac{n!}{k!(n-k)!}](https://latex.codecogs.com/svg.image?\bg_white&space;(&space;^{n}_{k})=&space;\frac{n!}{k!(n-k)!})

**PASCAL'S TRIANGLE:**
--

&nbsp; &nbsp; &nbsp; &nbsp; &nbsp; &nbsp;   (<sup>0</sup> C <sub>0</sub>)\
&nbsp; &nbsp; &nbsp; &nbsp;(<sup>1</sup> C <sub>1</sub>)  (<sup>1</sup> C <sub>1</sub>)\
&nbsp; &nbsp;(<sup>2</sup> C <sub>0</sub>) (<sup>2</sup> C <sub>1</sub>) (<sup>2</sup> C <sub>2</sub>)\
(<sup>3</sup> C <sub>0</sub>) (<sup>3</sup> C <sub>1</sub>) (<sup>3</sup> C <sub>2</sub>)(<sup>3</sup> C <sub>3</sub>)

&nbsp; &nbsp; &nbsp; &nbsp; &nbsp; &nbsp;(1)\
&nbsp; &nbsp; &nbsp; &nbsp; &nbsp;(1)  (1)\
&nbsp; &nbsp; &nbsp; &nbsp;(1) (2) (1)\
&nbsp; &nbsp; &nbsp;(1) (3) (3)(1)


**BINOMIAL THEOREM FOR NEGATIVE INTEGER EXPONENTS:**
--

![\frac{1}{(1+x)^{n}}= \sum_{k=0}^{\infty }(^{n+k-1}_{k})(-1)^{k}x^{k}](https://latex.codecogs.com/svg.image?\bg_white&space;\frac{1}{(1&plus;x)^{n}}=&space;\sum_{k=0}^{\infty&space;}(^{n&plus;k-1}_{k})(-1)^{k}x^{k})

-> this can be verified by expanding lhs using the std binomial formula and then the expansion can be easily summarized to rhs
